lib/Buckets/MapSeqs.i.dfy
@@ -1,0 +1,307 @@
+include "../Base/KeyType.s.dfy"
+include "../Base/Message.i.dfy"
+include "../Base/total_order.i.dfy"
+
+module MapSeqs {
+  import opened KeyType
+  import opened ValueMessage
+  import opened Sequences
+  import opened Lexicographic_Byte_Order
+  import opened Maps
+  import opened Options
+
+  protected function map_of_seqs(keys: seq<Key>, msgs: seq<Message>) : map<Key, Message>
+  requires |keys| == |msgs|
+  {
+    if |keys| == 0 then
+      map[]
+    else
+      map_of_seqs(DropLast(keys), DropLast(msgs))[Last(keys) := Last(msgs)]
+  }
+
+  function maximumKey(b: set<Key>) : Option<Key>
+  {
+    var m := Lexicographic_Byte_Order.maximumOpt(b);
+    if m.Some? then
+      assert |m.value| <= KeyType.MaxLen() as nat;
+      var k: Key := m.value;
+      Some(k)
+    else
+      None
+  } 
+
+  datatype SeqPair = SeqPair(keys: seq<Key>, msgs: seq<Message>)
+
+  protected function seqs_of_map(m: map<Key, Message>) : (res : SeqPair)
+  ensures |res.keys| == |res.msgs|
+  {
+    var keyOpt := maximumKey(m.Keys);
+    match keyOpt {
+      case None => SeqPair([], [])
+      case Some(key) => (
+        var m' := MapRemove1(m, key);
+        var SeqPair(keys', msgs') := seqs_of_map(m');
+        SeqPair(keys' + [key], msgs' + [m[key]])
+      )
+    }
+  }
+
+  lemma IsStrictlySorted_seqs_of_map(m: map<Key, Message>)
+  ensures IsStrictlySorted(seqs_of_map(m).keys)
+  {
+    var keyOpt := maximumKey(m.Keys);
+    match keyOpt {
+      case None => {
+        reveal_IsStrictlySorted();
+      }
+      case Some(key) => {
+        var m' := MapRemove1(m, key);
+        var SeqPair(keys', msgs') := seqs_of_map(m');
+        IsStrictlySorted_seqs_of_map(m');
+        StrictlySortedAugment(keys', key);
+      }
+    }
+  }
+
+  lemma MapMapsIndex(keys: seq<Key>, msgs: seq<Message>, i: int)
+  requires |keys| == |msgs|
+  requires 0 <= i < |keys|
+  requires IsStrictlySorted(keys)
+  ensures keys[i] in map_of_seqs(keys, msgs)
+  ensures map_of_seqs(keys, msgs)[keys[i]] == msgs[i]
+  {
+    if i == |keys| - 1 {
+    } else {
+      reveal_IsStrictlySorted();
+      //calc {
+      //  msgs[i];
+      //  {
+          MapMapsIndex(DropLast(keys), DropLast(msgs), i);
+      //  }
+      //  map_of_seqs(DropLast(keys), DropLast(msgs))[keys[i]];
+      //  map_of_seqs(DropLast(keys), DropLast(msgs))[Last(keys) := Last(msgs)][keys[i]];
+      //  map_of_seqs(keys, msgs)[keys[i]];
+      //}
+    }
+  }
+
+  lemma map_of_seqs_of_seqs_of_map(m: map<Key, Message>)
+  ensures
+    var a := seqs_of_map(m);
+    map_of_seqs(a.keys, a.msgs) == m
+  {
+    assume false;
+  }
+
+  lemma GetIndex(keys: seq<Key>, msgs: seq<Message>, key: Key)
+  returns (i: int)
+  requires |keys| == |msgs|
+  requires key in map_of_seqs(keys, msgs)
+  ensures 0 <= i < |keys|
+  ensures keys[i] == key
+  ensures msgs[i] == map_of_seqs(keys, msgs)[key]
+  {
+    if keys[|keys| - 1] == key {
+      i := |keys| - 1;
+    } else {
+      i := GetIndex(DropLast(keys), DropLast(msgs), key);
+    }
+  }
+
+  lemma GetIndexOfVal(keys: seq<Key>, msgs: seq<Message>, key: Key, m: Message)
+  returns (i: int)
+  requires |keys| == |msgs|
+  requires key in map_of_seqs(keys, msgs)
+  requires map_of_seqs(keys, msgs)[key] == m
+  ensures 0 <= i < |keys|
+  ensures keys[i] == key
+  ensures msgs[i] == m
+  {
+    if keys[|keys| - 1] == key && msgs[|msgs| - 1] == m {
+      i := |keys| - 1;
+    } else {
+      i := GetIndex(DropLast(keys), DropLast(msgs), key);
+    }
+  }
+
+  lemma lemma_maxkey_not_in_map_of_seqs_drop_last(keys: seq<Key>, msgs: seq<Message>)
+  requires |keys| == |msgs|
+  requires IsStrictlySorted(keys)
+  requires |keys| > 0
+  ensures keys[|keys| - 1] !in map_of_seqs(DropLast(keys), DropLast(msgs))
+  {
+    if keys[|keys| - 1] in map_of_seqs(DropLast(keys), DropLast(msgs)) {
+      var i := GetIndex(DropLast(keys), DropLast(msgs), keys[|keys| - 1]);
+      reveal_IsStrictlySorted();
+    }
+  }
+
+  lemma SeqsEqOfMapsEq(
+      keys: seq<Key>, msgs: seq<Message>,
+      keys': seq<Key>, msgs': seq<Message>)
+  requires IsStrictlySorted(keys)
+  requires IsStrictlySorted(keys')
+  requires |keys| == |msgs|
+  requires |keys'| == |msgs'|
+  requires map_of_seqs(keys, msgs) == map_of_seqs(keys', msgs')
+  ensures keys == keys'
+  ensures msgs == msgs'
+  {
+    if |keys| == 0 {
+      assert map_of_seqs(keys', msgs')
+          == map_of_seqs(keys, msgs)
+          == map[];
+      if 0 < |keys'| {
+        MapMapsIndex(keys', msgs', 0);
+        assert false;
+      }
+    } else {
+      var maxkey := Last(keys);
+      var maxval := Last(msgs);
+
+      MapMapsIndex(keys, msgs, |keys| - 1);
+      var i := GetIndex(keys', msgs', maxkey);
+
+      assert i == |keys'| - 1 by {
+        if i < |keys'| - 1 {
+          var maxkey' := Last(keys');
+          MapMapsIndex(keys', msgs', |keys'| - 1);
+          var j := GetIndex(keys, msgs, maxkey');
+          reveal_IsStrictlySorted();
+        }
+      }
+
+      assert Last(keys) == Last(keys');
+
+      assert IsStrictlySorted(DropLast(keys)) by { reveal_IsStrictlySorted(); }
+      assert IsStrictlySorted(DropLast(keys')) by { reveal_IsStrictlySorted(); }
+
+      calc {
+        map_of_seqs(DropLast(keys), DropLast(msgs));
+        {
+          lemma_maxkey_not_in_map_of_seqs_drop_last(keys, msgs);
+        }
+        MapRemove1(map_of_seqs(keys, msgs), maxkey);
+        MapRemove1(map_of_seqs(keys', msgs'), maxkey);
+        {
+          lemma_maxkey_not_in_map_of_seqs_drop_last(keys', msgs');
+        }
+        map_of_seqs(DropLast(keys'), DropLast(msgs'));
+      }
+
+      SeqsEqOfMapsEq(
+          DropLast(keys), DropLast(msgs),
+          DropLast(keys'), DropLast(msgs'));
+
+      calc {
+        keys;
+        DropLast(keys) + [Last(keys)];
+        DropLast(keys') + [Last(keys')];
+        keys';
+      }
+
+      calc {
+        msgs;
+        DropLast(msgs) + [Last(msgs)];
+        DropLast(msgs') + [Last(msgs')];
+        msgs';
+      }
+    }
+  }
+
+  lemma MapOfEmptySeq()
+  ensures map_of_seqs([], []) == map[]
+  ensures IsStrictlySorted([])
+  {
+    reveal_IsStrictlySorted();
+  }
+
+  lemma map_of_seqs_push_back(
+      keys: seq<Key>, msgs: seq<Message>, key: Key, msg: Message)
+  requires |keys| == |msgs|
+  requires IsStrictlySorted(keys)
+  requires forall k | k in keys :: lt(k, key)
+  ensures map_of_seqs(keys + [key], msgs + [msg])
+       == map_of_seqs(keys, msgs)[key := msg]
+  ensures key !in map_of_seqs(keys, msgs)
+  {
+    //reveal_BucketMapOfSeq();
+    if key in map_of_seqs(keys, msgs) {
+      var i := GetIndex(keys, msgs, key);
+      assert lt(keys[i], key);
+    }
+  }
+
+  lemma map_of_seqs_pop_front(
+      keys: seq<Key>, msgs: seq<Message>, i: int)
+  requires |keys| == |msgs|
+  requires 0 <= i < |keys|
+  requires IsStrictlySorted(keys)
+  ensures map_of_seqs(keys[i+1..], msgs[i+1..])[keys[i] := msgs[i]]
+       == map_of_seqs(keys[i..], msgs[i..])
+  ensures keys[i] !in map_of_seqs(keys[i+1..], msgs[i+1..])
+  {
+    var a := map_of_seqs(keys[i+1..], msgs[i+1..])[keys[i] := msgs[i]];
+    var b := map_of_seqs(keys[i..], msgs[i..]);
+    forall k | k in a
+    ensures k in b
+    ensures a[k] == b[k]
+    {
+      reveal_IsStrictlySorted();
+      if k == keys[i] {
+        MapMapsIndex(keys[i..], msgs[i..], 0);
+        assert a[k] == b[k];
+      } else {
+        var j := GetIndex(keys[i+1..], msgs[i+1..], k);
+        MapMapsIndex(keys[i..], msgs[i..], j+1);
+        assert a[k] == b[k];
+      }
+    }
+    forall k | k in b
+    ensures k in a
+    {
+      reveal_IsStrictlySorted();
+      var j := GetIndex(keys[i..], msgs[i..], k);
+      if j > 0 {
+        MapMapsIndex(keys[i+1..], msgs[i+1..], j-1);
+      } else {
+      }
+    }
+    if keys[i] in map_of_seqs(keys[i+1..], msgs[i+1..]) {
+      var j := GetIndex(keys[i+1..], msgs[i+1..], keys[i]);
+      reveal_IsStrictlySorted();
+      assert false;
+    }
+  }
+
+  lemma map_union_of_seq_concat(
+      keys1: seq<Key>, msgs1: seq<Message>,
+      keys2: seq<Key>, msgs2: seq<Message>)
+  requires |keys1| == |msgs1|
+  requires |keys2| == |msgs2|
+  requires IsStrictlySorted(keys1 + keys2)
+  ensures IsStrictlySorted(keys1)
+  ensures IsStrictlySorted(keys2)
+  ensures map_of_seqs(keys1, msgs1).Keys !! map_of_seqs(keys2, msgs2).Keys
+  ensures MapDisjointUnion(map_of_seqs(keys1, msgs1), map_of_seqs(keys2, msgs2))
+      == map_of_seqs(keys1 + keys2, msgs1 + msgs2)
+  {
+    assume false; // TODO
+  }
+
+  lemma eq_map_of_seqs(keys: seq<Key>, msgs: seq<Message>, bmap: map<Key, Message>)
+  requires IsStrictlySorted(keys)
+  requires Set(keys) == bmap.Keys
+  requires |keys| == |msgs|
+  requires forall i | 0 <= i < |keys| :: bmap[keys[i]] == msgs[i]
+  ensures bmap == map_of_seqs(keys, msgs)
+  {
+    assume false; // TODO
+  }
+
+  lemma key_sets_eq(keys: seq<Key>, msgs: seq<Message>)
+  requires |keys| == |msgs|
+  ensures Set(keys) == map_of_seqs(keys, msgs).Keys
+  {
+  }
+}
